test/tube/Hacl.Tube.fst
@@ -6,48 +6,108 @@ open FStar.Buffer
 open PaddedFileIO
 open SocketIO
 open Hacl.Constants
-
+open Hacl.Cast
+open Box.Ideal 
+module U64=FStar.UInt64
 type clock = u64
-type string = seq u8
+type str = buffer u8
 
+type boxtype = 
+  | BOX_CHACHA_POLY
+  | SECRETBOX_CHACHA_POLY
 
-type streamID = {
-     id: u64;
-     ts: u64;
+type streamID = b:buffer u8{length b = 16}
+
+type open_result = {
+  r: PaddedFileIO.fresult;
+  sid: streamID;
+  fs: PaddedFileIO.file_stat
 }
 
-type principals = {
-     pkA: seq u8;
-     pkB: seq u8
+val opened: PaddedFileIO.fresult -> PaddedFileIO.file_stat -> streamID -> Tot open_result
+let opened r fs sid = {r = r; sid = sid; fs = fs}
+
+(* TODO: make streamID less opaque:
+{
+     ty: boxtype;
+     ts: C.clock_t;
+     id: buffer u8;
 }
+*)
 
+assume val sent: FStar.HyperStack.mem -> pkA: seq u8 -> pkB: seq u8 -> sid:seq u8 -> file_stat -> (seq u8) -> GTot bool
 
-assume val sent: FStar.HyperStack.mem -> principals -> streamID -> file_stat -> (seq u8) -> GTot bool
-
-assume val file_send: file:string -> roundup:u64 ->
-       host:string -> port:u32 -> 
-       skA:buffer u8 -> pkA:buffer u8 -> pkB:buffer u8 ->
-           Stack (fresult * file_stat * streamID)
-	   (requires (fun _ -> True))
-	   (ensures  (fun h0 s h1 -> match s with 
-      	   	                   | FileOk,fs,sid ->
-				     let prins = {pkA = as_seq h0 pkA; pkB = as_seq h0 pkB} in
-				     file_content h0 fs = file_content h1 fs /\	
-				     sent h1 prins sid fs (file_content h0 fs)
-				   | _ -> true))
-
-assume val file_recv: port:u32 -> pkA:buffer u8 -> skB:buffer u8 -> pkB:buffer u8 -> Stack (fresult * file_stat * streamID)
-       	   (requires (fun _ -> True))
-	   (ensures  (fun h0 s h1 -> match s with 
-      	   	                   | FileOk,fs,sid ->
-				     let prins = {pkA = as_seq h0 pkA; pkB = as_seq h0 pkB} in
-				     sent h0 prins sid fs (file_content h1 fs)
-				   | _ -> true))
-
-
-
-val main: unit -> ST FStar.Int32.t
+val makeStreamID: unit -> StackInline streamID
   (requires (fun h -> True))
   (ensures  (fun h0 r h1 -> True))
-let main () =
-  C.exit_success
+let makeStreamID () = 
+    let b = create 0uy 16ul in
+    randombytes_buf b (U64.uint_to_t 16);
+    b
+
+val putU64: z:u64 -> b:buffer u8 -> StackInline unit
+  (requires (fun h -> live h b /\ length b = 8))
+  (ensures  (fun h0 r h1 -> live h1 b))
+let putU64 z b = 
+  let open Hacl.UInt64 in
+  b.(0ul) <- sint64_to_sint8 z;
+  b.(1ul) <- sint64_to_sint8 (z >>^ 8ul);
+  b.(2ul) <- sint64_to_sint8 (z >>^ 16ul);
+  b.(3ul) <- sint64_to_sint8 (z >>^ 24ul);
+  b.(4ul) <- sint64_to_sint8 (z >>^ 32ul);
+  b.(5ul) <- sint64_to_sint8 (z >>^ 40ul);
+  b.(6ul) <- sint64_to_sint8 (z >>^ 48ul);
+  b.(7ul) <- sint64_to_sint8 (z >>^ 56ul)
+
+val file_send: file:str -> roundup:u64 ->
+       host:str -> port:u32 -> 
+       skA:buffer u8 -> pkB:buffer u8 ->
+           Stack open_result
+	   (requires (fun _ -> True))
+	   (ensures  (fun h0 s h1 -> match s.r with 
+      	   	                   | FileOk ->
+				     let fs = s.fs in
+				     let sidb = s.sid in
+				     let pA = pubKey (as_seq h0 skA) in
+				     let pB = as_seq h0 pkB in
+				     let sid = as_seq h0 sidb in
+				     file_content h0 fs = file_content h1 fs /\	
+				     sent h1 pA pB sid fs (file_content h0 fs)
+				   | _ -> true))
+let file_send f r h p skA pkB =
+  let sid = makeStreamID() in
+  let fh = init_file_handle in
+  let fb = Buffer.create fh 1ul in
+  match (file_open_read_sequential f fb) with
+  | FileOk -> 
+      let fh = fb.(0ul) in
+      let s = init_socket in
+      let sb = Buffer.create s 1ul in
+     (match tcp_connect h p sb with
+      | SocketOk ->
+	  let s = sb.(0ul) in
+	  (match tcp_write_all s sid 8uL with
+	   | SocketOk -> opened FileOk fh.stat sid
+	   | SocketError -> opened FileError fh.stat sid)
+      | SocketError -> opened FileError fh.stat sid)
+  | FileError -> opened FileError fh.stat sid
+  
+
+
+val file_recv: port:u32 -> pkA:buffer u8 -> skB:buffer u8 -> Stack open_result
+       	   (requires (fun _ -> True))
+	   (ensures  (fun h0 s h1 -> match s.r with 
+      	   	                   | FileOk ->
+				     let fs = s.fs in
+				     let sidb = s.sid in
+				     let pA = as_seq h0 pkA in
+				     let pB = pubKey (as_seq h0 skB) in
+				     let sid = as_seq h0 sidb in
+				     sent h0 pA pB sid fs (file_content h1 fs)
+				   | _ -> true))
+let file_recv p pkA skB =
+ let sid = makeStreamID() in
+ let fh = init_file_handle in
+ opened FileError fh.stat sid
+
+
