test/tube/SocketIO.fsti
@@ -18,6 +18,7 @@ type sresult =
      | SocketOk: sresult
      | SocketError: sresult
 
+val init_socket: socket
 val tcp_connect: host: string -> port:u32 -> s:buffer socket -> Stack sresult
     (requires (fun _ -> True))
     (ensures  (fun h0 r h1 -> match r with 
@@ -37,15 +38,15 @@ val tcp_accept: l:socket -> s:buffer socket -> Stack sresult
 			      	let sh = get h1 s 0 in
 				current_state h1 sh = Open))
 
-val tcp_write_all: s:socket -> string -> len:u64 -> Stack bool
+val tcp_write_all: s:socket -> string -> len:u64 -> Stack sresult
     (requires (fun h0 -> current_state h0 s = Open))
-    (ensures  (fun _ r h1 -> r ==> current_state h1 s = Open))
+    (ensures  (fun _ r h1 -> r = SocketOk ==> current_state h1 s = Open))
 
-val tcp_read_all: s:socket -> buffer u8 -> len:u64 -> Stack bool
+val tcp_read_all: s:socket -> buffer u8 -> len:u64 -> Stack sresult
     (requires (fun h0 -> current_state h0 s = Open))
-    (ensures  (fun _ r h1 -> r ==> current_state h1 s = Open))
+    (ensures  (fun _ r h1 -> r = SocketOk ==> current_state h1 s = Open))
 
-val tcp_close: s:socket -> Stack bool
+val tcp_close: s:socket -> Stack sresult
     (requires (fun h0 -> current_state h0 s = Open))
-    (ensures  (fun _ r h1 -> r ==> current_state h1 s = Closed))
+    (ensures  (fun _ r h1 -> r = SocketOk ==> current_state h1 s = Closed))
 
